examples/GasSeparator/Requirements.thy
@@ -15,61 +15,68 @@ always2_inv_part (\<lambda> s. getPstate s p_ButtonPressControl' \<noteq> p_Butt
   (\<lambda> s2. getVarBool s2 v_AutoBtn' = True) (\<lambda> s2. getVarBool s2 v_filling' = True \<and> getVarBool s2 v_release' = True \<and> getVarBool s2 v_FillingLED' = True) s"
 
 definition R2 where "R2 s \<equiv>
- let trigger = (\<lambda> s2. let s1 = pred s2 in  (let s0 = pred s1 in toEnvP s0 \<and> getVarBool s0 v_filling' = False \<and> getVarBool s1 v_filling' = True)) in
+ let trigger = (\<lambda> s1.  (let s0 = pred s1 in toEnvP s0 \<and> getVarBool s0 v_filling' = False \<and> getVarBool s1 v_filling' = True)) in
   let final = (\<lambda> s3. getVarBool s3 v_Lfull' = True) in
   let release = (\<lambda> s4. getVarBool s4 v_EmergencyBtn' = True \<or> getVarBool s4 v_ThighAbnormally' = True \<or> getVarBool s4 v_PhighAbnormally' = True) in
   let invariant = (\<lambda> s5. let s4 = pred s5 in toEnvP s4 \<and>  getVarBool s4 v_filling' = True \<and> getVarBool s4 v_release' = True \<and> getVarBool s4 v_FillingLED' = True) in
   let reaction = (\<lambda> s5. getVarBool s5 v_filling' = False \<and> getVarBool s5 v_release' = False \<and> getVarBool s5 v_FillingLED' = False) in
-  EDTL_delay_true_part trigger final release invariant reaction s"
+  EDTL_trigger_prev_delay_true_part trigger final release invariant reaction s"
 
 definition Einv2 where "Einv2 s \<equiv>
- let trigger = (\<lambda> s2. let s1 = pred s2 in  (let s0 = pred s1 in toEnvP s0 \<and> getVarBool s0 v_filling' = False \<and> getVarBool s1 v_filling' = True)) in
+ let trigger = (\<lambda> s1.  (let s0 = pred s1 in toEnvP s0 \<and> getVarBool s0 v_filling' = False \<and> getVarBool s1 v_filling' = True)) in
   let final = (\<lambda> s3. getVarBool s3 v_Lfull' = True) in
   let release = (\<lambda> s4. getVarBool s4 v_EmergencyBtn' = True \<or> getVarBool s4 v_ThighAbnormally' = True \<or> getVarBool s4 v_PhighAbnormally' = True) in
   let invariant = (\<lambda> s5. let s4 = pred s5 in toEnvP s4 \<and>  getVarBool s4 v_filling' = True \<and> getVarBool s4 v_release' = True \<and> getVarBool s4 v_FillingLED' = True) in
   let reaction = (\<lambda> s5. getVarBool s5 v_filling' = False \<and> getVarBool s5 v_release' = False \<and> getVarBool s5 v_FillingLED' = False) in
-  EDTL_delay_true_inv_part (\<lambda> s. getPstate s p_AutoModeControl' = p_AutoModeControl's_filling') trigger final release invariant reaction s"
+  EDTL_trigger_prev_delay_true_inv_part
+     (\<lambda> s. getPstate s p_AutoModeControl' \<noteq> p_AutoModeControl's_filling')
+     (\<lambda> s. getPstate s p_AutoModeControl' = p_AutoModeControl's_filling')
+     trigger final release invariant reaction s"
 
 definition R3 where "R3 s \<equiv>
- let trigger = (\<lambda> s2. let s1 = pred s2 in  (let s0 = pred s1 in toEnvP s0 \<and> getVarBool s0 v_filling' = False \<and> getVarBool s1 v_filling' = True)) in
+ let trigger = (\<lambda> s1. (let s0 = pred s1 in toEnvP s0 \<and> getVarBool s0 v_filling' = False \<and> getVarBool s1 v_filling' = True)) in
   let final = (\<lambda> s3. getVarBool s3 v_Lfull' = True) in
   let release = (\<lambda> s4. getVarBool s4 v_ManualBtn' \<or> getVarBool s4 v_EmergencyBtn' \<or> getVarBool s4 v_ThighAbnormally' \<or> getVarBool s4 v_PhighAbnormally') in
   let invariant = (\<lambda> s5. True) in
   let reaction = (\<lambda> s5. getVarBool s5 v_DegasLED' = True \<and> getVarBool s5 v_heater' = True) in
-  EDTL_delay_true_part trigger final release invariant reaction s"
+  EDTL_trigger_prev_delay_true_part trigger final release invariant reaction s"
 
 definition Einv3 where "Einv3 s \<equiv>
- let trigger = (\<lambda> s2. let s1 = pred s2 in  (let s0 = pred s1 in toEnvP s0 \<and> getVarBool s0 v_filling' = False \<and> getVarBool s1 v_filling' = True)) in
+ let trigger = (\<lambda> s1. (let s0 = pred s1 in toEnvP s0 \<and> getVarBool s0 v_filling' = False \<and> getVarBool s1 v_filling' = True)) in
   let final = (\<lambda> s3. getVarBool s3 v_Lfull' = True) in
   let release = (\<lambda> s4. getVarBool s4 v_ManualBtn' \<or> getVarBool s4 v_EmergencyBtn' \<or> getVarBool s4 v_ThighAbnormally' \<or> getVarBool s4 v_PhighAbnormally') in
   let invariant = (\<lambda> s5. True) in
   let reaction = (\<lambda> s5. getVarBool s5 v_DegasLED' = True \<and> getVarBool s5 v_heater' = True) in
-  EDTL_delay_true_inv_part (\<lambda> s. getPstate s p_AutoModeControl' = p_AutoModeControl's_filling') trigger final release invariant reaction s"
+  EDTL_trigger_prev_delay_true_inv_part
+     (\<lambda> s. getPstate s p_AutoModeControl' \<noteq> p_AutoModeControl's_filling')
+     (\<lambda> s. getPstate s p_AutoModeControl' = p_AutoModeControl's_filling')
+      trigger final release invariant reaction s"
 
 definition R4 where "R4 s \<equiv>
-  let trigger = (\<lambda> s2. let s1 = pred s2 in (let s0 = pred s1 in toEnvP s0 \<and> getVarBool s0 v_DegasLED' = False \<and> getVarBool s1 v_DegasLED' = True)) in
+  let trigger = (\<lambda> s1. (let s0 = pred s1 in toEnvP s0 \<and> getVarBool s0 v_DegasLED' = False \<and> getVarBool s1 v_DegasLED' = True)) in
   let finalt = v_DEGASSING_TIMEOUT'TIMEOUT in
   let finale = (\<lambda> s3. getVarBool s3 v_Ldeg' = False) in
   let release = (\<lambda> s4. False) in
   let invariant = (\<lambda> s5. let s4 = pred s5 in toEnvP s4 \<and> getVarBool s4 v_DegasLED' = True) in
   let reaction = (\<lambda> s6. getVarBool s6 v_DegasLED' = False) in
-  EDTL_final_nontemporal_or_tau_delay_true_part finalt trigger finale release invariant reaction s"
+  EDTL_trigger_prev_final_nontemporal_or_tau_delay_true_part finalt trigger finale release invariant reaction s"
 
 definition Einv4 where "Einv4 s \<equiv>
-  let trigger = (\<lambda> s2. let s1 = pred s2 in (let s0 = pred s1 in toEnvP s0 \<and> getVarBool s0 v_DegasLED' = False \<and> getVarBool s1 v_DegasLED' = True)) in
+  let trigger = (\<lambda> s1. (let s0 = pred s1 in toEnvP s0 \<and> getVarBool s0 v_DegasLED' = False \<and> getVarBool s1 v_DegasLED' = True)) in
   let finalt = v_DEGASSING_TIMEOUT'TIMEOUT in
   let finale = (\<lambda> s3. getVarBool s3 v_Ldeg' = False) in
   let release = (\<lambda> s4. False) in
   let invariant = (\<lambda> s5. let s4 = pred s5 in toEnvP s4 \<and> getVarBool s4 v_DegasLED' = True) in
   let reaction = (\<lambda> s6. getVarBool s6 v_DegasLED' = False) in
-  EDTL_final_nontemporal_or_tau_delay_true_inv_part finalt
+  EDTL_trigger_prev_final_nontemporal_or_tau_delay_true_inv_part finalt
+      (\<lambda> s. getPstate s p_AutoModeControl' \<noteq> p_AutoModeControl's_degassing' \<or> ltime s p_AutoModeControl' > 1)
      (\<lambda> s. if getPstate s p_AutoModeControl' = p_AutoModeControl's_degassing' then ltime s p_AutoModeControl' else 0)
      (\<lambda> s. if getPstate s p_AutoModeControl' = p_AutoModeControl's_degassing' then ltime s p_AutoModeControl' - 1 else v_DEGASSING_TIMEOUT'TIMEOUT - 1)
      (\<lambda> s. if getPstate s p_AutoModeControl' = p_AutoModeControl's_degassing' then ltime s p_AutoModeControl' else 0)
      trigger finale release invariant reaction s"
 
 definition R5 where "R5 s \<equiv>
-  let trigger = (\<lambda> s2. let s1 = pred s2 in (let s0 = pred s1 in toEnvP s0 \<and> toEnvP s1 \<and> getVarBool s0 v_heater' = False \<and> getVarBool s1 v_heater' = True)) in
+  let trigger = (\<lambda> s1. (let s0 = pred s1 in toEnvP s0 \<and> toEnvP s1 \<and> getVarBool s0 v_heater' = False \<and> getVarBool s1 v_heater' = True)) in
   let finalt = v_HEATING_TIMEOUT'TIMEOUT in
   let finale = (\<lambda> s3. let s2 = pred s3 in toEnvP s2 \<and> getVarBool s3 v_Thigh' = True \<or> getVarBool s3 v_Phigh' = True \<or> getVarBool s2 v_DegasLED' = False) in
   let release = (\<lambda> s4. False) in
@@ -78,57 +85,62 @@ definition R5 where "R5 s \<equiv>
   EDTL_final_nontemporal_or_tau_delay_true_part finalt trigger finale release invariant reaction s"
 
 definition Einv5 where "Einv5 s \<equiv>
-  let trigger = (\<lambda> s2. let s1 = pred s2 in (let s0 = pred s1 in toEnvP s0 \<and> toEnvP s1 \<and> getVarBool s0 v_heater' = False \<and> getVarBool s1 v_heater' = True)) in
+  let trigger = (\<lambda> s1. (let s0 = pred s1 in toEnvP s0 \<and> toEnvP s1 \<and> getVarBool s0 v_heater' = False \<and> getVarBool s1 v_heater' = True)) in
   let finalt = v_HEATING_TIMEOUT'TIMEOUT in
   let finale = (\<lambda> s3. let s2 = pred s3 in toEnvP s2 \<and> getVarBool s3 v_Thigh' = True \<or> getVarBool s3 v_Phigh' = True \<or> getVarBool s2 v_DegasLED' = False) in
   let release = (\<lambda> s4. False) in
   let invariant = (\<lambda> s5. let s4 = pred s5 in toEnvP s4 \<and> getVarBool s4 v_heater' = True) in
   let reaction = (\<lambda> s6. getVarBool s6 v_heater' = False) in
-  EDTL_final_nontemporal_or_tau_delay_true_inv_part finalt
+  EDTL_trigger_prev_final_nontemporal_or_tau_delay_true_inv_part finalt
+     (\<lambda> s. getPstate s p_DegassingControl' \<noteq> p_DegassingControl's_heating' \<or> ltime s p_DegassingControl' > 1)
      (\<lambda> s. if getPstate s p_DegassingControl' = p_DegassingControl's_heating' then ltime s p_DegassingControl' else 0)
      (\<lambda> s. if getPstate s p_DegassingControl' = p_DegassingControl's_heating' then ltime s p_DegassingControl' - 1 else v_HEATING_TIMEOUT'TIMEOUT - 1)
      (\<lambda> s. if getPstate s p_DegassingControl' = p_DegassingControl's_heating' then ltime s p_DegassingControl' else 0)
      trigger finale release invariant reaction s"
 
 definition R6 where "R6 s \<equiv>
-  let trigger = (\<lambda> s2. let s1 = pred s2 in (let s0 = pred s1 in toEnvP s0 \<and> toEnvP s1 \<and> getVarBool s0 v_heater' = True \<and> getVarBool s1 v_heater' = False)) in
+  let trigger = (\<lambda> s1. (let s0 = pred s1 in toEnvP s0 \<and> toEnvP s1 \<and> getVarBool s0 v_heater' = True \<and> getVarBool s1 v_heater' = False)) in
   let finalt = v_ACCUMULATING_TIMEOUT'TIMEOUT in
   let finale = (\<lambda> s3. getVarBool s3 v_Phigh' = True) in
   let release = (\<lambda> s4. let s3 = pred s4 in toEnvP s3 \<and> getVarBool s3 v_DegasLED' = False) in
   let invariant = (\<lambda> s5. let s4 = pred s5 in toEnvP s5 \<and> getVarBool s4 v_release' = False) in
   let reaction = (\<lambda> s6. getVarBool s6 v_release' = True) in
-  EDTL_final_nontemporal_or_tau_delay_true_part finalt trigger finale release invariant reaction s"
+  EDTL_trigger_prev_final_nontemporal_or_tau_delay_true_part finalt trigger finale release invariant reaction s"
 
 definition Einv6 where "Einv6 s \<equiv>
-  let trigger = (\<lambda> s2. let s1 = pred s2 in (let s0 = pred s1 in toEnvP s0 \<and> toEnvP s1 \<and> getVarBool s0 v_heater' = True \<and> getVarBool s1 v_heater' = False)) in
+  let trigger = (\<lambda> s1. (let s0 = pred s1 in toEnvP s0 \<and> toEnvP s1 \<and> getVarBool s0 v_heater' = True \<and> getVarBool s1 v_heater' = False)) in
   let finalt = v_ACCUMULATING_TIMEOUT'TIMEOUT in
   let finale = (\<lambda> s3. getVarBool s3 v_Phigh' = True) in
   let release = (\<lambda> s4. let s3 = pred s4 in toEnvP s3 \<and> getVarBool s3 v_DegasLED' = False) in
   let invariant = (\<lambda> s5. let s4 = pred s5 in toEnvP s5 \<and> getVarBool s4 v_release' = False) in
   let reaction = (\<lambda> s6. getVarBool s6 v_release' = True) in
-  EDTL_final_nontemporal_or_tau_delay_true_inv_part finalt
+  EDTL_trigger_prev_final_nontemporal_or_tau_delay_true_inv_part finalt
+     (\<lambda> s. getPstate s p_ButtonPressControl' \<noteq> p_ButtonPressControl's_waiting' \<and> getPstate s p_EmergencyControl' \<in> {p_EmergencyControl's_autoMode', STOP} \<and>
+       getPstate s p_AutoModeControl' = p_AutoModeControl's_degassing' \<and> 
+       (getPstate s p_DegassingControl' \<noteq> p_DegassingControl's_accumulating' \<or> ltime s p_DegassingControl' > 1))
      (\<lambda> s. if getPstate s p_DegassingControl' = p_DegassingControl's_accumulating' then ltime s p_DegassingControl' else 0)
      (\<lambda> s. if getPstate s p_DegassingControl' = p_DegassingControl's_accumulating' then ltime s p_DegassingControl' - 1 else v_ACCUMULATING_TIMEOUT'TIMEOUT - 1)
      (\<lambda> s. if getPstate s p_DegassingControl' = p_DegassingControl's_accumulating' then ltime s p_DegassingControl' else 0)
      trigger finale release invariant reaction s"
 
 definition R7 where "R7 s \<equiv>
-  let trigger =  (\<lambda> s2. let s1 = pred s2 in (let s0 = pred s1 in toEnvP s0 \<and> toEnvP s1 \<and> getVarBool s0 v_release' = False \<and> getVarBool s1 v_release' = True)) in
+  let trigger =  (\<lambda> s1. (let s0 = pred s1 in toEnvP s0 \<and> getVarBool s1 v_DegasLED' \<and>  getVarBool s0 v_release' = False \<and> getVarBool s1 v_release' = True)) in
   let finalt = v_RELEASE_TIMEOUT'TIMEOUT in
   let finale = (\<lambda> s3. (let s2 = pred s3 in toEnvP s2 \<and> getVarBool s3 v_Plow' = False \<or> getVarBool s2 v_DegasLED' = False)) in
-  let release = (\<lambda> s4. False) in
+  let release = (\<lambda> s4. getVarBool s v_DegasLED' = False) in
   let invariant = (\<lambda> s5. let s4 = pred s5 in toEnvP s5 \<and> getVarBool s4 v_release' = True) in
   let reaction = (\<lambda> s6. getVarBool s6 v_release' = False) in
-  EDTL_final_nontemporal_or_tau_delay_true_part finalt trigger finale release invariant reaction s"
+  EDTL_trigger_prev_final_nontemporal_or_tau_delay_true_part finalt trigger finale release invariant reaction s"
 
 definition Einv7 where "Einv7 s \<equiv>
-  let trigger =  (\<lambda> s2. let s1 = pred s2 in (let s0 = pred s1 in toEnvP s0 \<and> toEnvP s1 \<and> getVarBool s0 v_release' = False \<and> getVarBool s1 v_release' = True)) in
+  let trigger = (\<lambda> s1. (let s0 = pred s1 in toEnvP s0 \<and> getVarBool s1 v_DegasLED' \<and>  getVarBool s0 v_release' = False \<and> getVarBool s1 v_release' = True)) in
   let finalt = v_RELEASE_TIMEOUT'TIMEOUT in
   let finale = (\<lambda> s3. (let s2 = pred s3 in toEnvP s2 \<and> getVarBool s3 v_Plow' = False \<or> getVarBool s2 v_DegasLED' = False)) in
-  let release = (\<lambda> s4. False) in
+  let release = (\<lambda> s4. getVarBool s v_DegasLED' = False) in
   let invariant = (\<lambda> s5. let s4 = pred s5 in toEnvP s5 \<and> getVarBool s4 v_release' = True) in
   let reaction = (\<lambda> s6. getVarBool s6 v_release' = False) in
-  EDTL_final_nontemporal_or_tau_delay_true_inv_part finalt
+  EDTL_trigger_prev_final_nontemporal_or_tau_delay_true_inv_part finalt
+     (\<lambda> s. getPstate s p_DegassingControl' \<noteq> p_DegassingControl's_releasing' \<or> ltime s p_DegassingControl' > 1)
      (\<lambda> s. if getPstate s p_DegassingControl' = p_DegassingControl's_releasing' then ltime s p_DegassingControl' else 0)
      (\<lambda> s. if getPstate s p_DegassingControl' = p_DegassingControl's_releasing' then ltime s p_DegassingControl' - 1 else v_RELEASE_TIMEOUT'TIMEOUT - 1)
      (\<lambda> s. if getPstate s p_DegassingControl' = p_DegassingControl's_releasing' then ltime s p_DegassingControl' else 0)
@@ -143,57 +155,62 @@ definition Einv8 where "Einv8 s \<equiv>
   (\<lambda> s1. getVarBool s1 v_release' = True \<and> getVarBool s1 v_DegasLED' = True) (\<lambda> s2. getVarBool s2 v_Plow' = False) (\<lambda> s2. getVarBool s2 v_heater' = True) s"
 
 definition R9 where "R9 s \<equiv>
- let trigger = (\<lambda> s2. let s1 = pred s2 in (let s0 = pred s1 in toEnvP s0 \<and> toEnvP s1 \<and> getVarBool s0 v_DegasLED' = False \<and> getVarBool s1 v_DegasLED' = True)) in
+ let trigger = (\<lambda> s1. (let s0 = pred s1 in toEnvP s0 \<and> toEnvP s1 \<and> getVarBool s0 v_DegasLED' = False \<and> getVarBool s1 v_DegasLED' = True)) in
   let final = (\<lambda> s3. let s2 = pred s3 in toEnvP s2 \<and> getVarBool s2 v_DegasLED' = False) in
   let release = (\<lambda> s4. getVarBool s4 v_ManualBtn' = True) in
   let invariant = (\<lambda> s5. True) in
   let reaction = (\<lambda> s5. getVarBool s5 v_emptying' = True \<and> getVarBool s5 v_inert' = True) in
-  EDTL_delay_true_part trigger final release invariant reaction s"
+  EDTL_trigger_prev_delay_true_part trigger final release invariant reaction s"
 
 definition Einv9 where "Einv9 s \<equiv>
- let trigger = (\<lambda> s2. let s1 = pred s2 in (let s0 = pred s1 in toEnvP s0 \<and> toEnvP s1 \<and> getVarBool s0 v_DegasLED' = False \<and> getVarBool s1 v_DegasLED' = True)) in
+ let trigger = (\<lambda> s1. (let s0 = pred s1 in toEnvP s0 \<and> toEnvP s1 \<and> getVarBool s0 v_DegasLED' = False \<and> getVarBool s1 v_DegasLED' = True)) in
   let final = (\<lambda> s3. let s2 = pred s3 in toEnvP s2 \<and> getVarBool s2 v_DegasLED' = False) in
   let release = (\<lambda> s4. getVarBool s4 v_ManualBtn' = True) in
   let invariant = (\<lambda> s5. True) in
   let reaction = (\<lambda> s5. getVarBool s5 v_emptying' = True \<and> getVarBool s5 v_inert' = True) in
-  EDTL_delay_true_inv_part (\<lambda> s. getVarBool s v_DegasLED' = True) trigger final release invariant reaction s"
+  EDTL_trigger_prev_delay_true_inv_part (\<lambda> s. getVarBool s v_DegasLED' = False) (\<lambda> s. getVarBool s v_DegasLED' = True)
+     trigger final release invariant reaction s"
 
 definition R10 where "R10 s \<equiv>
- let trigger = (\<lambda> s2. let s1 = pred s2 in (let s0 = pred s1 in toEnvP s0 \<and> toEnvP s1 \<and> getVarBool s0 v_inert' = False \<and> getVarBool s1 v_inert' = True)) in
+ let trigger = (\<lambda> s1. (let s0 = pred s1 in toEnvP s0 \<and> toEnvP s1 \<and> getVarBool s0 v_inert' = False \<and> getVarBool s1 v_inert' = True)) in
   let final = (\<lambda> s3. getVarBool s3 v_Llow' = False) in
   let release = (\<lambda> s4. False) in
   let invariant = (\<lambda> s5. let s4 = pred s5 in toEnvP s5 \<and> getVarBool s4 v_inert' = True) in
   let reaction = (\<lambda> s5. getVarBool s5 v_inert' = False) in
-  EDTL_delay_true_part trigger final release invariant reaction s"
+  EDTL_trigger_prev_delay_true_part trigger final release invariant reaction s"
 
 definition Einv10 where "Einv10 s \<equiv>
- let trigger = (\<lambda> s2. let s1 = pred s2 in (let s0 = pred s1 in toEnvP s0 \<and> toEnvP s1 \<and> getVarBool s0 v_inert' = False \<and> getVarBool s1 v_inert' = True)) in
+ let trigger = (\<lambda> s1. (let s0 = pred s1 in toEnvP s0 \<and> toEnvP s1 \<and> getVarBool s0 v_inert' = False \<and> getVarBool s1 v_inert' = True))in
   let final = (\<lambda> s3. getVarBool s3 v_Llow' = False) in
   let release = (\<lambda> s4. False) in
   let invariant = (\<lambda> s5. let s4 = pred s5 in toEnvP s5 \<and> getVarBool s4 v_inert' = True) in
   let reaction = (\<lambda> s5. getVarBool s5 v_inert' = False) in
-  EDTL_delay_true_inv_part (\<lambda> s. getVarBool s v_inert' = True)  trigger final release invariant reaction s"
+  EDTL_trigger_prev_delay_true_inv_part
+      (\<lambda> s. getPstate s p_EmergencyControl' \<noteq> p_EmergencyControl's_emptying' \<and> getPstate s p_AutoModeControl' \<noteq> p_AutoModeControl's_emptying')
+     (\<lambda> s. getVarBool s v_inert' = True)  trigger final release invariant reaction s"
 
 definition R11 where "R11 s \<equiv>
- let trigger = (\<lambda> s2. let s1 = pred s2 in (let s0 = pred s1 in toEnvP s0 \<and> toEnvP s1 \<and> getVarBool s0 v_emptying' = False \<and> getVarBool s1 v_emptying' = True)) in
+ let trigger = (\<lambda> s1. (let s0 = pred s1 in toEnvP s0 \<and> toEnvP s1 \<and> getVarBool s0 v_emptying' = False \<and> getVarBool s1 v_emptying' = True)) in
   let final = (\<lambda> s3. getVarBool s3 v_Lempty' = True) in
   let release = (\<lambda> s4. False) in
   let invariant = (\<lambda> s5. let s4 = pred s5 in toEnvP s5 \<and> getVarBool s4 v_emptying' = True) in
   let reaction = (\<lambda> s5. getVarBool s5 v_emptying' = False) in
-  EDTL_delay_true_part trigger final release invariant reaction s"
+  EDTL_trigger_prev_delay_true_part trigger final release invariant reaction s"
 
 definition Einv11 where "Einv11 s \<equiv>
- let trigger = (\<lambda> s2. let s1 = pred s2 in (let s0 = pred s1 in toEnvP s0 \<and> toEnvP s1 \<and> getVarBool s0 v_emptying' = False \<and> getVarBool s1 v_emptying' = True)) in
+ let trigger =  (\<lambda> s1. (let s0 = pred s1 in toEnvP s0 \<and> toEnvP s1 \<and> getVarBool s0 v_emptying' = False \<and> getVarBool s1 v_emptying' = True)) in
   let final = (\<lambda> s3. getVarBool s3 v_Lempty' = True) in
   let release = (\<lambda> s4. False) in
   let invariant = (\<lambda> s5. let s4 = pred s5 in toEnvP s5 \<and> getVarBool s4 v_emptying' = True) in
   let reaction = (\<lambda> s5. getVarBool s5 v_emptying' = False) in
-  EDTL_delay_true_inv_part
+  EDTL_trigger_prev_delay_true_inv_part
+     (\<lambda> s. getPstate s p_EmergencyControl' \<noteq> p_EmergencyControl's_emptying' \<and> getPstate s p_AutoModeControl' \<noteq> p_AutoModeControl's_emptying')
      (\<lambda> s. getPstate s p_EmergencyControl' = p_EmergencyControl's_emptying' \<or> getPstate s p_AutoModeControl' = p_AutoModeControl's_emptying')
      trigger final release invariant reaction s"
 
 definition R12 where "R12 s \<equiv>
- let trigger = (\<lambda> s2. let s1 = pred s2 in toEnvP s1 \<and> getVarBool s1 v_SafetyLED' = False \<and> getVarBool s1 v_EmergencyLED' \<and> getVarBool s1 v_DegasLED' = False) in
+ let trigger = (\<lambda> s2. let s1 = pred s2 in toEnvP s1 \<and> getVarBool s1 v_SafetyLED' = False \<and> getVarBool s1 v_EmergencyLED' \<and>
+   getVarBool s1 v_DegasLED' = False) in
   let final = (\<lambda> s3. let s2 =pred s3 in toEnvP s2 \<and> getVarBool s2 v_emptying' = True \<and> getVarBool s3 v_Lempty' = True) in
   let release = (\<lambda> s4. getVarBool s4 v_ManualBtn' \<or> getVarBool s4 v_SafetyStopBtn' \<or> getVarBool s4 v_EmergencyBtn' \<or> getVarBool s4 v_ThighAbnormally'
      \<or> getVarBool s4 v_PhighAbnormally' = True) in
@@ -226,12 +243,12 @@ always2_inv_part (\<lambda> s. getPstate s p_ButtonPressControl' \<noteq> p_Butt
   (\<lambda> s2. getVarBool s2 v_SafetyLED' = True) s"
 
 definition R14 where "R14 s \<equiv>
- let trigger = (\<lambda> s2. let s1 = pred s2 in  (let s0 = pred s1 in toEnvP s0 \<and> getVarBool s0 v_SafetyLED' = False \<and> getVarBool s1 v_SafetyLED' = True)) in
-  let final = (\<lambda> s2. let s1 = pred s2 in  (let s0 = pred s1 in toEnvP s0 \<and> getVarBool s0 v_purge' = True \<and> getVarBool s1 v_purge' = False)) in
+ let trigger = (\<lambda> s1. (let s0 = pred s1 in toEnvP s0 \<and> getVarBool s0 v_SafetyLED' = False \<and> getVarBool s1 v_SafetyLED' = True)) in
+  let final = (\<lambda> s1. (let s0 = pred s1 in toEnvP s0 \<and> getVarBool s0 v_purge' = True \<and> getVarBool s1 v_purge' = False)) in
   let release = (\<lambda> s4. getVarBool s4 v_EmergencyBtn' = True \<or> getVarBool s4 v_ThighAbnormally' = True \<or> getVarBool s4 v_PhighAbnormally' = True) in
   let invariant = (\<lambda> s5. let s4 = pred s5 in toEnvP s4 \<and> getVarBool s4 v_SafetyLED' = True) in
   let reaction = (\<lambda> s5. getVarBool s5 v_SafetyLED' = False) in
-  EDTL_delay_true_part trigger final release invariant reaction s"
+  EDTL_trigger_prev_final_prev_delay_true_part trigger final release invariant reaction s"
 
 definition Einv14 where "Einv14 s \<equiv>
  let trigger = (\<lambda> s2. let s1 = pred s2 in  (let s0 = pred s1 in toEnvP s0 \<and> getVarBool s0 v_SafetyLED' = False \<and> getVarBool s1 v_SafetyLED' = True)) in
@@ -246,20 +263,28 @@ definition Einv14 where "Einv14 s \<equiv>
 definition R15 where "R15 s \<equiv>
  let trigger = (\<lambda> s2. let s1 = pred s2 in toEnvP s1 \<and> getVarBool s1 v_AutoLED' = True
      \<and> (getVarBool s2 v_SafetyStopBtn' \<or> getVarBool s2 v_EmergencyBtn' \<or> getVarBool s2 v_ThighAbnormally' \<or> getVarBool s2 v_PhighAbnormally')) in
-  let final = (\<lambda> s2. let s1 = pred s2 in  (let s0 = pred s1 in toEnvP s0 \<and> getVarBool s0 v_emptying' = True \<and> getVarBool s1 v_emptying' = False)) in
+  let final = (\<lambda> s1.  (let s0 = pred s1 in toEnvP s0 \<and> getVarBool s0 v_emptying' = True \<and> getVarBool s1 v_emptying' = False)) in
   let release = (\<lambda> s4. False) in
   let invariant = (\<lambda> s5. True) in
   let reaction = (\<lambda> s5. getVarBool s5 v_purge' = True) in
-  EDTL_delay_true_part trigger final release invariant reaction s"
+  EDTL_final_prev_delay_true_part trigger final release invariant reaction s"
 
 definition Einv15 where "Einv15 s \<equiv>
  let trigger = (\<lambda> s2. let s1 = pred s2 in toEnvP s1 \<and> getVarBool s1 v_AutoLED' = True
      \<and> (getVarBool s2 v_SafetyStopBtn' \<or> getVarBool s2 v_EmergencyBtn' \<or> getVarBool s2 v_ThighAbnormally' \<or> getVarBool s2 v_PhighAbnormally')) in
-  let final = (\<lambda> s2. let s1 = pred s2 in  (let s0 = pred s1 in toEnvP s0 \<and> getVarBool s0 v_emptying' = True \<and> getVarBool s1 v_emptying' = False)) in
+  let final = (\<lambda> s1.  (let s0 = pred s1 in toEnvP s0 \<and> getVarBool s0 v_emptying' = True \<and> getVarBool s1 v_emptying' = False)) in
   let release = (\<lambda> s4. False) in
   let invariant = (\<lambda> s5. True) in
   let reaction = (\<lambda> s5. getVarBool s5 v_purge' = True) in
-  EDTL_delay_true_inv_part (\<lambda> s. getPstate s p_EmergencyControl' = p_EmergencyControl's_emptying') trigger final release invariant reaction s"
+  EDTL_final_prev_delay_true_inv_part
+     (\<lambda> s. (getPstate s p_EmergencyControl' \<noteq> p_EmergencyControl's_purge' \<or> ltime s p_EmergencyControl' > 1) \<and>
+        (getPstate s p_AutoModeControl' \<noteq> STOP \<or> 
+          getPstate s p_ButtonPressControl' \<notin> {p_ButtonPressControl's_waitingForEmptying', p_ButtonPressControl's_waitingForStageCompletion'}) \<and>
+        (getPstate s p_AutoModeControl' \<noteq> p_AutoModeControl's_filling'))
+    (\<lambda> s. (getPstate s p_EmergencyControl' = p_EmergencyControl's_purge' \<and> ltime s p_EmergencyControl' = 1) \<and>
+        (getPstate s p_AutoModeControl' = STOP \<and> 
+          getPstate s p_ButtonPressControl' = p_ButtonPressControl's_waitingForEmptying'))
+     (\<lambda> s. getPstate s p_EmergencyControl' = p_EmergencyControl's_emptying') trigger final release invariant reaction s"
 
 definition R16 where "R16 s \<equiv>
 P1_2_part 1 (\<lambda> s1. getVarBool s1 v_AutoLED' = True) 
@@ -276,18 +301,20 @@ P1_2_inv_part 1 (\<lambda> s. getPstate s p_ButtonPressControl' \<noteq> p_Butto
 definition R17 where "R17 s \<equiv>
 let final =  v_PURGE_TIMEOUT'TIMEOUT in
 let delay = 1 in
-let trigger =  (\<lambda> s2. let s1 = pred s2 in let s0 = pred s1 in  toEnvP s0 \<and> getVarBool s0 v_purge' =False \<and> getVarBool s1 v_purge' = True) in
+let trigger = (\<lambda> s1. let s0 = pred s1 in  toEnvP s0 \<and> getVarBool s0 v_purge' =False \<and> getVarBool s1 v_purge' = True) in
 let invariant = (\<lambda> s3. let s2 = pred s3 in toEnvP s2 \<and> getVarBool s2 v_purge' = True \<and> getVarBool s2 v_release' = True) in
 let reaction = (\<lambda> s3. getVarBool s3 v_purge' = False \<and> getVarBool s3 v_release' = False) in
-EDTL_release_false_final_tau_delay_tau_part final delay trigger invariant reaction s"
+EDTL_trigger_prev_release_false_final_tau_delay_tau_part final delay trigger invariant reaction s"
 
 definition Einv17 where "Einv17 s \<equiv>
 let final =  v_PURGE_TIMEOUT'TIMEOUT in
 let delay = 1 in
-let trigger =  (\<lambda> s2. let s1 = pred s2 in let s0 = pred s1 in  toEnvP s0 \<and> getVarBool s0 v_purge' =False \<and> getVarBool s1 v_purge' = True) in
+let trigger = (\<lambda> s1. let s0 = pred s1 in  toEnvP s0 \<and> getVarBool s0 v_purge' =False \<and> getVarBool s1 v_purge' = True) in
 let invariant = (\<lambda> s3. let s2 = pred s3 in toEnvP s2 \<and> getVarBool s2 v_purge' = True \<and> getVarBool s2 v_release' = True) in
 let reaction = (\<lambda> s3. getVarBool s3 v_purge' = False \<and> getVarBool s3 v_release' = False) in
-EDTL_release_false_final_tau_delay_tau_inv_part final delay
+EDTL_trigger_prev_release_false_final_tau_delay_tau_inv_part final delay
+   (\<lambda> s. (getPstate s p_ButtonPressControl' \<noteq> p_ButtonPressControl's_purge' \<or> ltime s p_ButtonPressControl' > 1) \<and> 
+    (getPstate s p_EmergencyControl' \<noteq> p_ButtonPressControl' \<or> ltime s p_ButtonPressControl' > 2))
    (\<lambda> s. if getPstate s p_ButtonPressControl' = p_ButtonPressControl's_purge' then ltime s p_ButtonPressControl' - 1
      else if getPstate s p_EmergencyControl' = p_EmergencyControl's_purge' then ltime s p_EmergencyControl' - 2 else v_PURGE_TIMEOUT'TIMEOUT - 2)
    (\<lambda> s. if getPstate s p_ButtonPressControl' = p_ButtonPressControl's_purge' then ltime s p_ButtonPressControl'
@@ -363,19 +390,21 @@ definition Einv23 where "Einv23 s \<equiv>
 always_inv_part (\<lambda> s1. getVarBool s1 v_filling' = False \<and> getVarBool s1 v_DegasLED' = False \<or> getVarBool s1 v_emptying'=  False) s"
 
 definition R24 where "R24 s \<equiv>
-let trigger =  (\<lambda> s2. let s1 = pred s2 in let s0 = pred s1 in toEnvP s0 \<and> getVarBool s0 v_purge' = True \<and> getVarBool s1 v_purge' = False) in
+let trigger =  (\<lambda> s1. let s0 = pred s1 in toEnvP s0 \<and> getVarBool s0 v_purge' = True \<and> getVarBool s1 v_purge' = False) in
 let final = (\<lambda> s3. False) in
 let release = (\<lambda> s4. getVarBool s4 v_AutoBtn' = True) in
 let invariant = (\<lambda> s3. let s2 = pred s3 in toEnvP s2 \<and> getVarBool s2 v_filling' = False \<and> getVarBool s2 v_DegasLED' = False \<and> getVarBool s2 v_emptying' = False) in
 let reaction = (\<lambda> s3. True) in
- EDTL_delay_true_part trigger final release invariant reaction s"
+ EDTL_trigger_prev_delay_true_part trigger final release invariant reaction s"
 
 definition Einv24 where "Einv24 s \<equiv>
-let trigger =  (\<lambda> s2. let s1 = pred s2 in let s0 = pred s1 in toEnvP s0 \<and> getVarBool s0 v_purge' = True \<and> getVarBool s1 v_purge' = False) in
+let trigger =  (\<lambda> s1. let s0 = pred s1 in toEnvP s0 \<and> getVarBool s0 v_purge' = True \<and> getVarBool s1 v_purge' = False) in
 let final = (\<lambda> s3. False) in
 let release = (\<lambda> s4. getVarBool s4 v_AutoBtn' = True) in
 let invariant = (\<lambda> s3. let s2 = pred s3 in toEnvP s2 \<and> getVarBool s2 v_filling' = False \<and> getVarBool s2 v_DegasLED' = False \<and> getVarBool s2 v_emptying' = False) in
 let reaction = (\<lambda> s3. True) in
- EDTL_delay_true_inv_part (\<lambda> s. getPstate s p_ButtonPressControl' = p_ButtonPressControl's_waiting') trigger final release invariant reaction s"
+ EDTL_trigger_prev_delay_true_inv_part
+    (\<lambda> s. getPstate s p_ButtonPressControl' \<noteq> p_ButtonPressControl's_waiting')
+    (\<lambda> s. getPstate s p_ButtonPressControl' = p_ButtonPressControl's_waiting') trigger final release invariant reaction s"
 
 end
